기본적으로는 True, False 만 알 수 있고, '정의되지 않은 관계'는 'refine'으로 제한한다.

src/01-01-Introduction/YCSCS1.Introduction.Semantic.HistoryOfCompiler.SpeedCoding.fst
@@ -6,10 +6,10 @@ module YCSCS1.Introduction.Semantic.HistoryOfCompiler.SpeedCoding
 
 type program_language_t =
 | SpeedCoding
-| Assembly
+| HandwrittenAssembly
 
 type program_kind_t =
-| Interpreted
+| InterpreterRequired
 | Compiled
 
 type time_t =
@@ -18,21 +18,66 @@ type time_t =
 
 type program_t =
 | SpeedCodingInterpreter
-| Product: lang: program_language_t -> program_t
+| IBM704Program: (lang: program_language_t) -> program_t
+| TodayProgram: (kind: program_kind_t) -> program_t
+
+type program_size_t =
+| Byte300
 
 //---|
+
 
 let get_program_kind (program: program_t) : program_kind_t =
   match program with
   | SpeedCodingInterpreter -> Compiled
-  | Product lang ->
+  | IBM704Program lang ->
+  begin
     match lang with
-    | SpeedCoding -> Interpreted
-    | Assembly -> Compiled
+    | SpeedCoding -> InterpreterRequired
+    | HandwrittenAssembly -> Compiled
+  end
+  | TodayProgram kind -> kind
 
-let is_less_productive_than (pk_l pk_r: program_kind_t) : bool =
+let get_time (program: program_t) : time_t =
+  match program with
+  | SpeedCodingInterpreter
+  | IBM704Program _ -> Year1953
+  | TodayProgram _ -> Today
+
+private let is_less_productive_than_core (pk_l pk_r: program_kind_t) : bool =
   match pk_l, pk_r with
-  | Compiled, Interpreted -> true
+  | Compiled, InterpreterRequired -> true
   | _ -> false
+
+let is_less_productive_than (program_l program_r: program_t) : 
+  Pure bool (requires (get_time program_l) = (get_time program_r)) (ensures fun _ -> True)
+  =
+  is_less_productive_than_core (get_program_kind program_l) (get_program_kind program_r)
+
+private let is_slower_than_core (pk_l pk_r: program_kind_t) : bool =
+  match pk_l, pk_r with
+  | InterpreterRequired, Compiled -> true
+  | _ -> false
+
+let is_slower_than (program_l program_r: program_t) : 
+  Pure bool (requires (get_time program_l) = (get_time program_r)) (ensures fun _ -> True)
+  =
+  is_slower_than_core (get_program_kind program_l) (get_program_kind program_r)
+
+let get_program_size (program: program_t{SpeedCodingInterpreter? program}) : program_size_t =
+  match program with
+  | SpeedCodingInterpreter -> Byte300
+
+let is_size_trouble (size: program_size_t) (time: time_t) : bool =
+  match size, time with
+  | Byte300, Year1953 -> true
+  | Byte300, Today -> false
+
+let is_well_known_language 
+  (lang: program_language_t{SpeedCoding? lang}) 
+  (time: time_t{Today? time})
+  : bool =
+  match lang, time with
+  | SpeedCoding, Today -> false
 
 // </snippet:history-of-compiler-ibm704>
